\documentclass{article}

\usepackage{amsmath}
\usepackage{amssymb}
\usepackage{amsthm}
\usepackage[margin = 2.54cm]{geometry}
% \usepackage{tikz}

\newtheorem{lemma}{Lemma}
\newtheorem{definition}[lemma]{Definition}
\newtheorem{prop}[lemma]{Proposition}

\begin{document}
We jump to the proposition.
\begin{prop}[Multiple integration]
  If $f(x)$ is smooth enough, we have
  \begin{equation}
    I_n f(x) \mathrel{:=}
    I_0^{x_0} \prod_{i = 1}^n (I_0^x) f(x) =
    \int_0^{x_0} \frac{(x_0 - x)^n}{n!} f(x) \, \mathrm{d} x,
  \end{equation}
  where $n \in \mathbb{N}$.
\end{prop}
\begin{proof}
  We extend the definition of $I$ as
  \begin{equation}
    I_{n, m} f(x) \mathrel{:=}
    I_0^{x_0} g_m(x) \prod_{i = 1}^n (I_0^x) f(x),
  \end{equation}
  where $g_m(x)$ is defined as
  \begin{equation}
    g_m(x) \mathrel{:=} \frac{(x_0 - x)^m}{m!},
  \end{equation}
  and we have
  \[\begin{aligned}
    I_{n, m} f(x) &=
    \int_0^{x_0} g_m(x)
    \underbrace{\int_0^x \! \cdots \int_0^x}_n f(x)
    \, \underbrace{\mathrm{d} x \cdots \mathrm{d} x}_{n + 1} \\
    &= g_{m + 1}(x)
    \underbrace{\int_0^x \! \cdots \int_0^x}_n f(x)
    \, \underbrace{\mathrm{d} x \cdots \mathrm{d} x}_{n} \biggr\rvert_{x_0}^0 +
    \int_0^{x_0} \! g_{m + 1}(x) \underbrace{\int_0^x \! \cdots \int_0^x}_{n - 1} f(x)
    \, \underbrace{\mathrm{d} x \cdots \mathrm{d} x}_{n} \\
    &= \int_0^{x_0} g_{m + 1}(x) \underbrace{\int_0^x \! \cdots \int_0^x}_{n - 1}
    f(x) \, \underbrace{\mathrm{d} x \cdots \mathrm{d} x}_{n} \\
    &= I_{n - 1, m + 1} f(x) \\
    &= \cdots \\
    &= I_{0, m + n} f(x) \\
    &= \int_0^{x_0} g_{m + n}(x) f(x) \, \mathrm{d} x.
  \end{aligned}\]
  Also, note that $I_n f(x) = I_{n, 0} f(x)$, which implies
  $I_n f(x) = I_{0, n} f(x)$, completing the proof.
\end{proof}
\end{document}